Zcash/Circuits.lean
@@ -81,6 +81,7 @@ import Zcash.Circuits.Ecc.Chip
 import Zcash.Circuits.Action.Circuit
 import Zcash.Circuits.Action.Bundle
 import Zcash.Circuits.Action.RealBases
+import Zcash.Circuits.Fixtures.ProjectSemantics
 
 /-!
 # Ironwood circuits
